Implement `FromBytes()` by `method`.
This removes `FromBytes2()` and, instead, solves the problem of
executing the function on large sequences using Dafny's `by method`
syntax.  That is verified to match the functional description.

src/dafny/util/int.dfy
@@ -252,7 +252,8 @@ module Int {
      }
 
     // Convert an arbitrary sized unsigned integer into a sequence of 1 or more
-    // bytes in big endian notation.
+    // bytes in big endian notation.  This is naturally a tail recursive
+    // function.
     function {:tailrecursion true} ToBytes(v:nat) : (r:seq<u8>)
     ensures |r| > 0 {
         // Extract the byte
@@ -266,36 +267,41 @@ module Int {
 
     // Convert a given sequence of zero or more bytes into an arbitrary sized
     // unsigned integer.  If the empty sequence is given, then zero is returned.
+    // This is implemented by method to ensure large sequences can be converted
+    // without overflowing the stack.
     function FromBytes(bytes:seq<u8>) : (r:nat) {
         if |bytes| == 0 then 0
-        else if |bytes| == 1 then bytes[0] as nat
         else
             var last := |bytes| - 1;
             var byte := bytes[last] as nat;
             var msw := FromBytes(bytes[..last]);
             (msw * 256) + byte
+    } by method {
+        r := 0;
+        for i := 0 to |bytes|
+        invariant r == FromBytes(bytes[..i]) {
+            var ith := bytes[i] as nat;
+            r := (r * 256) + ith;
+            assert r == (FromBytes(bytes[..i]) * 256) + ith;
+            LemmaFromBytes(bytes,i);
+        }
+        // Dafny needs help here :)
+        assert bytes[..|bytes|] == bytes;
+        // Done
+        return r;
     }
 
-    // Convert a given sequence of zero or more bytes into an arbitrary sized
-    // unsigned integer.  If the empty sequence is given, then zero is returned.
-    // A divide-and-conquer approach is used to limit the maximum stack depth to
-    // be log(|bytes|).
-    function FromBytes2(bytes:seq<u8>) : (r:nat) {
-        if |bytes| == 0 then 0
-        else if |bytes| == 1 then bytes[0] as nat
-        else
-            var pivot := |bytes| / 2;
-            var high := bytes[..pivot];
-            var low := bytes[pivot..];
-            var msw := FromBytes2(high);
-            var lsw := FromBytes2(low);
-            var factor := Pow(2,|low|*8);
-            (msw * factor) + lsw
-    }
-
-    lemma {:verify false} LemmaFromBytes2(bytes:seq<u8>)
-    ensures FromBytes(bytes) == FromBytes2(bytes) {
-
+    // Lemma connecting FromBytes at an arbitrary position within a sequence.
+    lemma LemmaFromBytes(bytes:seq<u8>,i:nat)
+    requires 0 <= i < |bytes|
+    ensures FromBytes(bytes[..i+1]) == (FromBytes(bytes[..i]) * 256) + bytes[i] as nat {
+        if i != 0 {
+            var cons := bytes[..i+1];
+            var tail := bytes[..i];
+            var head := bytes[i];
+            // For reasons unknown, Dafny cannot figure this out for itself.
+            assert (cons == tail + [head]);
+        }
     }
 
     // Sanity check that going to/from bytes gives identical result.
@@ -310,15 +316,18 @@ module Int {
     requires |bytes| > 0 && (|bytes| == 1 || bytes[0] != 0)
     ensures ToBytes(FromBytes(bytes)) == bytes { }
 
-    // Lemma to help connect the expected byte length of a natural number.  If
-    // we have a bound for that number, then its bytelength is also a bound.
+    // Lemma to help connect the expected byte length of two natural numbers.
+    // For example, if one number is less than another then its byte sequence
+    // will not be larger (though could be the same length).
     lemma LemmaLengthToBytes(n: nat, m: nat)
     requires n <= m
-    ensures |ToBytes(n)| <= |ToBytes(m)| {
+    ensures |ToBytes(n)| <= |ToBytes(m)| {}
 
-    }
-
-    // Another lemma to help connect expected byte length after coercions.
+    // Lemma to help connect the expected byte length of a natural number
+    // through coecion.  Specifically, converting a byte sequence into a number
+    // and then back again yields a byte sequence that is not longer than the
+    // original.  Observer, however, that it can be shorter if there are leading
+    // zeros in the original byte sequence.
     lemma LemmaLengthFromBytes(n: nat, bytes: seq<u8>)
     requires n == FromBytes(bytes)
     ensures bytes == [] || |ToBytes(n)| <= |bytes| {
